
$a(b + c) = ab + ac$

$a + b$
$f. x. (x^{f^a})^{f^{b}}$

$\hat{e} = [1][2](-1)$

$\hat{e} = \sqrt[2]{1}$

$\hat{e} = [1][2](\{f\} \to \{x\} \to f \to [x]f \to x)$
$\hat{e} = [1](\{x\} \to 2 \to [x]2 \to x)$
$\hat{e} = \{x\} [1](2 \to [x]2 \to x)$

$\hat{e} = \{x\} \to 1^{x^2 \to x}$

$\hat{e} = \{x\} \to 1^{\log_{x^2} x}$





$\hat{e} = \{x\} \to 1^{2^{-1}\{x\}}$

$\hat{e} = 1^{1/2}$






$1 = 1^{(4 \to 2)2}$


$e_1e_2$
$f.(f^{e_1})^{e_2}$
$1^{(4 \to 2) + (9 \to 3)}$

$1^{2((4 \to 2) + (9 \to 3))}$

$e_1 = 1^{4 \to 2}$
$e_2 = 1^{4 \to -2}$

$e_1^2 = 1$
$e_2^2 = 1$
$e_1e_2 = -e_2e_1$
$e_1 = -e_2e_1e_2$

$e_1 = 1^{2^{-1}}$
$\sqrt{1}\sqrt{1} = (-1)\sqrt{1}\sqrt{1}$
$1 = (-1)\sqrt{1}\sqrt{1}$
$\sqrt{1}\sqrt{1} = -1$

$\{x\} \to \{y\} \to (\sqrt{1}\{x\} \sqrt{1}\{y\} = -1)$
 



$0^{-1}$
$(f.x.x)^{\{f\} \to \{x\} \to f \to x^f \to x}$
$\{x\}\to 1 \to x$

$f.(\{x\} \to 1 \to x)(2f)$
$\{x\} \to f.(1 \to x)(2f)$
$\{x\} \to 2(1\to x)$

$f.(\{x\} \to 1 \to x)((f.x.x)f)$
$f.(\{x\} \to 1 \to x)(x.x)$
$\{x\} \to f.(1 \to x)1$
$\{x\} \to f.x$




$e_1 = \hat{e}\{0^{-1}\}$
$e_1 = 1^{0^{-2} \to 0^{-1}}$
$e_1 = 1^{(\{x\} \to 2(1 \to x)) \to (\{x\} \to 1 \to x)}$

if we merge:

$e_1 = \{x\} \to 1^{2(1 \to x) \to 1 \to x}$
$2(1\to x) \mapsto 1$
$(1 \to x) \mapsto 2^{-1}$
$x \mapsto 1^{2^{-1}}$
$e_1 = \{x\} \to \hat{e} \to x$

