$2^{-1}$
$(f\to x\to (x^f)^f)^{f\to x^f \to x}$
$x^{f \to x \to (x^f)^f} \to x$

$-1 = f \to x^f \to x$
$\frac{1}{2} = x^2\to x$

$e^{\pi i} = -1$
$\pi i = e.-1$
$\pi = (e. -1)i^{-1}$

$i^2 = -1$
$2 = i.-1$

$i^{-1}$
$i^{f\to x^f \to x}$
$x^i \to x$

$\nabla = d\to f \to x \to d^{-1}((x + d)^f - x^f)$

$\exp = f \Rightarrow f^{\epsilon^\nabla}$
$\exp = f \Rightarrow x \to (y^\epsilon \to y)((x + \epsilon)^f - x^f)$

$e = 1^{\exp}$
$e = 1^{f \Rightarrow x \to (y^\epsilon \to y)((x + \epsilon)^f - x^f)}$

$\pi = (e. -1)(x^i \to x)$
$\pi = (1^{f\Rightarrow x\to(y^\epsilon \to y)((x + \epsilon)^f - x^f)} \to f\to x^f \to x)(x^i \to x)$
$\exp(i\pi) = -1$
$\exp = i\pi \to -1$
$i\pi = -1 \leftarrow \exp$


$i^2 = -1$

$i^{x \to (x^2 = -1)} = \aleph$
$i \in x \to (x^2 = -1)$
$I = x\to (x^2 = -1)$

$i^2 = -1$



$2i = -1$
$i = -1 \leftarrow 2$

$2i$
$2(-1 \leftarrow 2)$
$-1$





$x.i (ix) = a.ab.b$
$x.i(ix) = x.xy.y$

$i(i1) = 1y.y$
$i = i1.1y.y$

$x.i(ix) = x.xy.y$
$x.(i(ix) = xy.y)$
$x.(i = ix.xy.y)$
$i = x.(xy.y \leftarrow i)$


$x.(i = x.(xy.y \leftarrow i))$

$2i$
$x.2i$
$x.(f.y.f(fy))i$
$x.y.i(iy)$
$x.i(ix)$
$x.i(xy.y \leftarrow i)$
$x.xy.y$
$-1$



$2i$
$(f.x.f(fx))(i1.1y.y)$
$x.(i1.1y.y)((i1.1y.y)x)$
$x.i(ix)$






$

$x.(i(ix) = xy.y)$
$x.(i = ix.xy.y)$
$x.i = x.n;nx.xy.y$
$x.(i = ix. xy. y)$



$i1(i1)(1(2)) = 2$
$i1 = i1.1y.y$
$(i1.1y.y)(i1)(1(2)) = 2$
$(1y.y)(1(2)) = 2$
$2 = 2$
$\aleph\quad\checkmark$

$x.2i = x.-1$
$x.(f.y.f (fy))i = x.-1$
$x.y.i(iy) = x.-1$
$x.y.i(iy) = x.y.yz.z$
$x.y.i((n;n0.0b.b)y) = x.y.yz.z$
$x.y.i()





$-1x(xy) = y$
$-1x = y \leftarrow xy$
$-1 = x \to (y \leftarrow xy)$


$a\to (c \leftarrow b) = c \leftarrow ba$


$-1x(xy) = y$
$-1x = xy.y$
$-1 = x.xy.y$


$x.(i = ix.y)$
$i = x.(y \leftarrow i)$

$x.i(ix) = x.xy.y$
$x.i = x.ix.xy.y$


$ax = b$
$x = b \leftarrow a$

"$x$ is the thing that when you pass to $a$, it gives back $b$"

$(-1)f(fx) \Leftrightarrow x$


# GA in LC

$2\hat{e} = 1$
$\hat{e} = 1 \leftarrow 2$

$(f.x.f (fx))\hat{e} = x.x$
$x.\hat{e}(\hat{e}x) = x.x$
$x. \hat{e}(\hat{e}x) = x.x$
$x.\hat{e}x = x.x \leftarrow \hat{e}$
$x.\hat{e} = x \rightarrow (1 \leftarrow \hat{e})$

$\hat{e} = 1 \rightarrow (1 \leftarrow \hat{e})$
$2\hat{e}$
$x.\hat{e}(\hat{e}x)$
$1 \to \hat{e}(1 \leftarrow \hat{e})$
$1 \rightarrow 1$

$(-1)x(xy) = y$

$(y^x)^{x^{-1}} = y$

$i^2 = -1$

$f^{-1 \times i} = (f^{i})^{f^{-1}}$




$(f^2)^{f^1}$
$


$x^{f^{i + (-1)\times i}} = (x^{f^{(-1)\times i}})^{f^{i}}$
$x^{f^{i + (-1)\times i}} = (x^{(f^{i})^{f^{-1}}})^{f^{i}}$
$x^1 = (x^{(f^{-1})^{f^i}})^{f^i}$




$x = if((if((-1)f))x)$


$(-1 = x.(xy \rightarrow y))$
$2i = -1$
$(f.x.f(fx))i = -1$
$x.i(ix) = -1$
$x.y.i(ix) = x.y.(xy \rightarrow y)$
$x.y.i = x.y.(xi \rightarrow xy \rightarrow y)$

$x.y.i(ix) = x.y.a.(ay \to a)$
$x.y.ix = x.y.((a.(ay \to a)) \leftarrow i)$
$x.y.i = x.y.(x \to ((a. (ay \to a)) \leftarrow i)))$
$i = (-1 \leftarrow 2)$



$f.x.-1 = f.x.(f \rightarrow fx \to x)$

$(-1)\times i$
$f.(-1)f(if)$
$f.([a] \to [ab] \to [b])f(if)$
$[a] \mapsto f$
$[ab] \mapsto if$
$f[b] \mapsto if$
$[b] \mapsto (if \leftarrow f)$

$([ai] \to [ab] \to [b])f \leftarrow f)$
$[ai] \mapsto f$
$[b] \mapsto x$
$[a] \mapsto (i \to f)$
$[ab] \mapsto (i \to f)x$


$f.(f \to if \to (if \leftarrow f))f(if)$
$f.(if \to (if \leftarrow f))(if)$
$f.(if \leftarrow f)$
$S = f.(if \leftarrow f)$
$x.S = x.f.((f \to (i \to f)x \to x) \leftarrow f)$


$i + (-1)\times i$
$f.x.if(((-1)\times i)fx)$
$f.x.if(Sfx)$
$f.x.([ai] \to [ab] \to [b])f(Sfx)$
$[ai] \mapsto f$
$[a] \mapsto (i \to f)$
$[ab] \mapsto Sfx$
$[b] \mapsto (Sfx \leftarrow a)$
$f.x.(Sfx \leftarrow (i \rightarrow f)) = 0$
$f.x.(f.((f \to (i \to f)[a] \to [a]) \leftarrow f)fx \leftarrow (i \to f)) = 0$
$(i \to f)[a] \mapsto x$
$[a] \mapsto (x \leftarrow (i \to f))$
$f.x.((x \leftarrow (i \to f)) \leftarrow (i \to f)) = f.x.x$
$f.x.(x \leftarrow (i \to f)) = f.x.(i \to f)x$
$f.x.x = f.x.(i \to f)(i \to f)x$
$f.x.x = f.x.(i \to f)(i \to f)x$

$(([xi] \rightarrow [xy] \rightarrow [y]) \to x.x)(x.x)$
$[xi] \mapsto x.x$
$[x] \mapsto (i \to x.x)$

$y.S = y.(i \to x.x)y \to y$
$y.S((i \to x.x)y) = y.y$
$y.S





$a.-1 = a.b.(ba \to a)$

$-1 \times i$
$f.(-1)f(if)$
$f.(-1)f((-1 \leftarrow 2)f)$
$f.(b.(b[a] \to [a]))f((-1 \leftarrow 2)f)$
$f.(f[a] \to [a])((-1 \leftarrow 2)f)$
$f[a] \mapsto (-1 \leftarrow 2)f$
$[a] \mapsto (-1 \leftarrow 2)f \leftarrow f$
$f.(-1 \leftarrow 2)f \leftarrow f$



$g.x.(-1 \leftarrow 2)g((f.(-1 \leftarrow 2)f \leftarrow f)gx)$
$g.x.(-1 \leftarrow 2)g(((-1 \leftarrow 2)g \leftarrow g)x)$
$g.x.ig((ig \leftarrow g)x)$


$g.x.(x^{g^i \leftarrow g})^{g^i}$


$a.b.(b^{a^i \leftarrow a})^{a^i} = a.b.b$
$b.(b^{1\leftarrow 1}) = b.b$

$1 \leftarrow 1 = 1$



$(b^{a^i \leftarrow a})^{a^i} = b$
$b^{a^i \leftarrow a} = b^{a^{-i}}$
$b^{a^i} = b^{(a^{-ia})}$

$a^{i} = a^{-ia}$

$3^i = 3^{-3i}$


$2^i = (-2^{2i})$





$S = ((-1 \leftarrow 2)g \leftarrow g)x$
$x \rightarrow S =(-1 \leftarrow 2)g \leftarrow g$
$g(x \to S) = (-1 \leftarrow 2)g$
$g \rightarrow g(x \to S) = -1 \leftarrow 2$
$2(g \to g(x \to S)) = -1$
$a.(g \to g(x \to S))((g \to g(x \to S))a)$

# 

$i + (-i)$

$f.x.-1 = f.x.(f \to fx \to x)$

$2i = -1$
$i = -1 \leftarrow 2$

$(-1)\times i$
$f.(-1)(if)$
$f.(-1)((-1 \leftarrow 2)f)$
$a.b.f.(a \to ab \to b)((-1 \leftarrow 2)f)$
$b.S = b.f.(if \rightarrow ifb \to b)$

$S = i + (-1)\times i$
$S = f.x.if(((-1)\times i)fx)$
$b.S = b.f.x.if((f. (if \to ifb \to b))fx)$
$b.S = b.f.x.if((if \to ifb \to b)x)$
$b.f.(if \to if) = b.f.(if \to if(ifb \to b))$
$b \to (i \leftarrow 2) \to 2 \to 2 = b \to (i \leftarrow 2) \to 2 \to 2(2b \to b)$
$2(2b \to b)$
$f.(2b\to b)((2b\to b)f)$
$2b.(2b \to b)b$

$b \to 2 = b\to 2b \to (2b \to b)b$
$





$a - a = 0$
$([x][f]a)[f](-a) = [x][f]0$
$([x][f]a)[f](-a) = [x]$
$[x][f]a = [x][f]a$
$\aleph$

$$\large e^{i\pi} = -1$$
$$\large i \pi = e \to -1$$
$$\large \pi = i^{-1}(e \to -1)$$
$$\large e = 1^{\exp}$$

$$\exp = f; d. x. (x + d)^f - x^f$$


$$\small \pi = (-1 \leftarrow 2)^{-1}(1^{\{f\} \to \nabla f} \to -1)$$

$(-1 \leftarrow 2)^{-1}$
$(-1 \leftarrow 2)^{f \Rightarrow x \Rightarrow f \to fx \to x}$
$x \Rightarrow (-1 \leftarrow 2) \rightarrow (-1 \leftarrow 2)x \to x$

$\pi = (\dagger \leftarrow e)i^{\dagger}$



# Classification

- Symbols: $a$, $b$, $c$.
- Functions: $a. x$ 
- Application: $f[x]$

### Inverses

- Forward restriction:
$$f[a] = b$$
$$f = a \to b$$
- Backward restriction:
$$f[a] = b$$
$$a = b \leftarrow f$$
- Scoped restriction:
$$a.x = a.y$$
$$x = \{a\} \rightarrow y$$



$f \Rightarrow x \rightarrow \dagger[0 \leftarrow 2]( f[x + (0 \leftarrow 2)] + f[x]\dagger)$

$\beta = f \Rightarrow x \rightarrow \dagger \epsilon \times \Delta f \epsilon$
$\Delta = f \rightarrow d \rightarrow x \rightarrow f(x + d) + \dagger fx$
$\epsilon = 0 \leftarrow 2$
$\dagger = \{f\} \rightarrow \{x\} \rightarrow f \rightarrow fx \rightarrow x$

$\beta = f \Rightarrow x \to \dagger \epsilon \times (f(x + \epsilon) - fx)$
$\epsilon = 0 \leftarrow 2$
$\dagger = \{f\} \to \{x\} \to f \to fx \to x$


$\exp = f \Rightarrow x\rightarrow \epsilon^\dagger((x + \epsilon)^f - x^f)$
$\epsilon = 0^{2^\dagger}$

$\epsilon^2 = 0$
$\epsilon = 0^{2^{-1}}$


$(0 \leftarrow 2) = (-1)(2)0$

$2^x = 5$
$x = \log_2 5$

$x = {_2}5$

$\epsilon = \sqrt{0}$


# Classification

- Functions: $a. x$ 
- Application: $x^f$

### Inverses

- Forward restriction:
$$f a = b$$
$$f = b_a$$
$$a^{b_a} = b$$
- Backward restriction:
$$a^f = b$$
$$a = {^f}b$$
$${^fb}^f = $$
- Scoped restriction:
$$a.x = a.y$$
$$x = a; y$$

$(0 \leftarrow 2) = (-1)(2)0$
$0 \leftarrow 2 = (-1)[2][0]$
$0 \leftarrow 2 = (\{f\} \to \{x\} \to f \to fx \to x)[2][0]$
$0 \leftarrow 2 = (2 \to 2[0] \to 0)$
$(0 \leftarrow 2)[2][2[0]] = 0$
$a[b \leftarrow a] = (b \leftarrow a)[a][a[b]] = b$
$b \leftarrow a = (-1)[a][b]$
$f[a] = b$
$f = a \to b$
$a = f \to f[b] \to b$

$a = 2$
$f = 3$
$b = 8$

$f[a] = b$
$3[2] = 8$
$3 = 2 \to 8$
$2 = (-1)[3][8]$
$2 = (\{f\} \to \{x\} \to f \to f[x] \to x)[3][8]$
$\{f\} \mapsto 3$
$\{f[x]\} \mapsto 8$
$\{x\} \mapsto (8 \leftarrow 3)$
$2 = 8 \leftarrow 3$

$(-1)[f][f[x]] = x$
$(f[x] \leftarrow f) = x$

$\hat{e} = 1 \leftarrow 2$
$e_1 \in \hat{e}$

$f[x] = y$
$x \in \{t \mid f[t] = y\}$
$f \ni x \to y$

$f???$
$f = \{f[t]\}$

For example:

$f = x.2x$
$f[n] = \{0, 2, 4, 6, 8, \dots\}$
(for $\mathbb{N}$ inputs)

$\{t \mid f[t] = y\}$

$s = \{1, 2, 3\}$
$f = x \mapsto \{a^2 \mid a \in x\}$

$(\times) := n.m.f.n(mf)$
$(\times) := (n, m, f) \mapsto \{n[a] \mid a \in \{m[b] \mid b \in f\}\}$
$(\times) := n \mapsto m \mapsto f \mapsto \{n[a] \mid a \in \{m[b] | b \in f\}\}$

Are functions sets?

$\hat{e}^2 = 1$
$(f \to x \to f [f[x]])[\hat{e}] = x \to x$
$x \to \hat{e}[\hat{e}[x]] = x \to x$
$x \to \hat{e} = x \to \hat{e}[x] \to x$
$\hat{e} = \{x\} \to x \to \hat{e}[x] \to x$
$\hat{e} = a \Rightarrow \{x\} \to x \to a[x] \to x$

$\hat{e} = (-1)[2][0]$
$\hat{e} = (\{f\} \to \{x\} \to f \to f[x] \to x)[2][0]$
$\hat{e} = (\{x\} \to 2 \to 2[x] \to x)[2][0]$

$\hat{e} = \{x\} \to (2[x] \to x)[1]$

$\hat{e}\{1\} = (2[1] \to 1)[1]$
$\hat{e}\{1\} = (1 \to 1)[1] = 1$

$\hat{e}\{\aleph\} = (2[\aleph] \to 1)[1]$

$x\to \aleph[\aleph[x]]$
$x \to \aleph[(a \to b \to a)x]$
$x \to \aleph[b \to x]$
$x \to (c \to d \to c)[b \to x]$
$x \to d \to b \to x$

$\hat{e}\{2\} = (4 \to 1)[1]$

$x. \hat{e}\{2\}[\hat{e}\{2\}[x]]$
$x. (4 \to 1)[1][(4 \to 1)[1][x]] = x.y.x y$
$x.(4 \to 1)[1][1 \leftarrow 4][x]]$
$x.(1 \leftarrow 4)[(1 \leftarrow 4)[x]] = x.y.x[y]$
$(1 \leftarrow 4)[x]$
$x.(1 \leftarrow 4) = x.((1 \leftarrow 4)[x] \to y.x[y])$
$\hat{e}\{2\} = x.(\hat{e}\{2\}[x] \to 1[x])$
$\hat{e}[2] = x.(\hat{e}[2] \to 1)$
$\{x\} \to \hat{e}\{2\} = \{x\} \to x \to \hat{e}\{2\} \to 1$
$\{x\} \to (\hat{e}\{2\} = x \to \hat{e}\{2\} \to 1)$
$\{x\} \to (\hat{e}\{2\}[x] = \hat{e}\{2\} \to 1)$
$\{x\} \to (x = (\hat{e}\{2\} \to 1) \leftarrow \hat{e}\{2\})$


$\hat{e}^2 = 1$
$2[\hat{e}] = 1$
$\hat{e} = 1 \leftarrow 2$

$\hat{e} = \{x\} \to (2[x] \to x)[1]$

$\hat{e} = (1 \leftarrow 2)$

$(1 + \hat{e})^2$
$(1 + \hat{e})(1 + \hat{e})$
$1 + \hat{e} + \hat{e} + \hat{e}^2$
$2 + \hat{e}$

$df'(\mathbf{v}) = f(\mathbf{v} + d) - f(v)$
$dv^{f^\nabla} = (v + d)^f - v^f$
$v^{f^\nabla} = d^{-1}((v + d)^f - v^f)$
$f^\nabla = \log_v(d^{-1}((v + d)^f - v^f))$
$\nabla = \log_f (\log_v(d^{-1}((v + d)^f - v^f)))$
$\nabla = \{d\}.\log_f(\log_v((d^{-1}((v + d)^f - v^f)))$

$\nabla = \{d\}.{_{{_f}v}}(d^{-1}((v + d)^f - v^f))$

